finished upto bit ops. Regs and Actions to be done next, followed by proof of simulation and proof of compiler

Syntax.v
@@ -1,276 +1,192 @@
 Require Export Bool Ascii String List Psatz PeanoNat.
+Require Export Guru.Lib.Library.
 Require Export Guru.Lib.Word Guru.Lib.WordProperties Guru.Lib.EclecticLib.
 
 Global Set Implicit Arguments.
 Global Set Asymmetric Patterns.
 
+Import ListNotations.
+
 Global Open Scope string_scope.
 Global Open Scope nat_scope.
 Global Open Scope list_scope.
 
-Inductive Kind :=
-| Bool   : Kind
-| Bit    : nat -> Kind
-| Struct : list (string * Kind) -> Kind
-| Array  : nat -> Kind -> Kind.
+Inductive UniBoolOp: Set :=
+| Not: UniBoolOp.
 
-Axiom cheat: forall t, t.
+Inductive CABoolOp: Set :=
+| And: CABoolOp
+| Xor: CABoolOp.
 
-Section KindDec.
-  Local Notation contra k1 k2 := (right (fun H : k1 = k2 => match match H in (_ = a) return match a with
-                                                                                            | k1 => True
-                                                                                            | _ => False
-                                                                                            end with
-                                                                  | eq_refl => I
-                                                                  end return False with
-                                                            end)).
+Inductive UniBitOp: nat -> nat -> Set :=
+| Inv n: UniBitOp n n
+| TruncLsb msb lsb: UniBitOp (msb + lsb) lsb
+| TruncMsb msb lsb: UniBitOp (msb + lsb) msb
+| UAnd n: UniBitOp n 1
+| UOr n: UniBitOp n 1
+| UXor n: UniBitOp n 1.
 
-  Fixpoint Kind_dec k1: forall k2: Kind, {k1 = k2} + {k1 <> k2} :=
-    match k1 with
-    | Bool => fun k2 => match k2 with
-                        | Bool => left eq_refl
-                        | Bit n => contra Bool (Bit n)
-                        | Struct ls => contra Bool (Struct ls)
-                        | Array n k => contra Bool (Array n k)
-                        end
-    | Bit n => fun k2 => match k2 with
-                         | Bool => contra (Bit n) Bool
-                         | Bit n1 => match Nat.eq_dec n n1 with
-                                     | left pf => left (match match pf in (_ = a) return (a = n) with
-                                                              | eq_refl => eq_refl
-                                                              end with
-                                                        | eq_refl => eq_refl
-                                                        end)
-                                     | right pf => right (fun H : Bit n = Bit n1 =>
-                                                            match pf match H in (_ = a) return (n = match a with
-                                                                                                    | Bit n0 => n0
-                                                                                                    | _ => n
-                                                                                                    end) with
-                                                                    | eq_refl => eq_refl
-                                                                    end return False with
-                                                            end)
+Inductive BinSign := SignSS | SignSU | SignUU.
 
-                                     end
-                         | Struct ls => contra (Bit n) (Struct ls)
-                         | Array n' k => contra (Bit n) (Array n' k)
-                         end
-    | Struct ls => fun k2 => match k2 with
-                             | Bool => contra (Struct ls) Bool
-                             | Bit n => contra (Struct ls) (Bit n)
-                             | Struct ls' => match list_eq_dec (prod_dec string_dec Kind_dec) ls ls' with
-                                             | left pf => left match match pf in (_ = a) return (a = ls) with
-                                                                     | eq_refl => eq_refl
-                                                                     end with
-                                                            | eq_refl => eq_refl
-                                                            end
-                                             | right n => right (fun H : Struct ls = Struct ls' =>
-                                                                   match n match H in (_ = a) return (ls = match a with
-                                                                                                           | Struct l => l
-                                                                                                           | _ => ls
-                                                                                                           end) with
-                                                                           | eq_refl => eq_refl
-                                                                           end return False with
-                                                                   end)
-                                             end
-                             | Array n k => contra (Struct ls) (Array n k)
-                             end
-    | Array n k => fun k2 => match k2 with
-                             | Bool => contra (Array n k) Bool
-                             | Bit n' => contra (Array n k) (Bit n')
-                             | Struct ls => contra (Array n k) (Struct ls)
-                             | Array n' k' =>
-                                 match Nat.eq_dec n n' with
-                                 | left e =>
-                                     match Kind_dec k k' with
-                                     | left pf =>
-                                         left
-                                           match match e in (_ = a) return (a = n) with
-                                                 | eq_refl => eq_refl
-                                                 end with
-                                           | eq_refl =>
-                                               match match pf in (_ = a) return (a = k) with
-                                                     | eq_refl => eq_refl
-                                                     end with
-                                               | eq_refl => eq_refl
-                                               end
-                                           end
-                                     | right pf =>
-                                         right
-                                           (fun H : Array n k = Array n' k' =>
-                                              match pf match H in (_ = a) return (k = match a with
-                                                                                      | Array _ k0 => k0
-                                                                                      | _ => k
-                                                                                      end) with
-                                                      | eq_refl => eq_refl
-                                                      end return False with
-                                              end)
-                                     end
-                                 | right pf =>
-                                     right
-                                       (fun H : Array n k = Array n' k' =>
-                                          match pf match H in (_ = a) return (n = match a with
-                                                                                  | Array n1 _ => n1
-                                                                                  | _ => n
-                                                                                  end) with
-                                                  | eq_refl => eq_refl
-                                                  end return False with
-                                          end)
-                                 end
-                             end
-    end.
-End KindDec.
+Inductive BinBitOp: nat -> nat -> nat -> Set :=
+| Sub n: BinBitOp n n n
+| Div n: BinBitOp n n n
+| Rem n: BinBitOp n n n
+| Sll n m: BinBitOp n m n
+| Srl n m: BinBitOp n m n
+| Sra n m: BinBitOp n m n
+| Concat msb lsb: BinBitOp msb lsb (msb + lsb).
 
-Section DiffTuple.
-  Variable A: Type.
-  Variable Convert: A -> Type.
-  Fixpoint DiffTuple (ls: list A) := match ls return Type with
-                                     | nil => Empty_set
-                                     | a :: xs => (Convert a * DiffTuple xs)%type
-                                     end.
-End DiffTuple.
+Inductive CABitOp: Set :=
+| Add: CABitOp
+| Mul: CABitOp
+| Band: CABitOp
+| Bxor: CABitOp.
 
-Section SameTuple.
-  Variable T: Type.
-  Fixpoint SameTuple n := match n return Type with
-                          | 0 => Empty_set
-                          | S m => (T * SameTuple m)%type
-                          end.
-End SameTuple.
+Inductive BinBitBoolOp: nat -> nat -> Set :=
+| LessThan n: BinBitBoolOp n n.
 
-Section KindInd.
-  Variable P: Kind -> Type.
-  Variable pBool: P Bool.
-  Variable pBit: forall n, P (Bit n).
-  Variable pStruct: forall ls: list (string * Kind), (fix help ls := match ls return Type with
-                                                                     | nil => unit: Type
-                                                                     | (_, k) :: xs => (P k * help xs)%type
-                                                                     end) ls -> P (Struct ls).
-  Variable pArray: forall n k, P k -> P (Array n k).
+Section Phoas.
+  Variable ty: Kind -> Type.
 
-  Fixpoint KindCustomInd (k: Kind): P k :=
-    match k return P k with
-    | Bool => pBool
-    | Bit n => pBit n
-    | Struct ls => pStruct ls ((fix help2 ls :=
-                                  match ls return ((fix help (ls' : list (string * Kind)) : Type := match ls' with
-                                                                                                    | nil => unit
-                                                                                                    | (_, k) :: xs => (P k * help xs)%type
-                                                                                                    end) ls) with
-                                  | nil => tt
-                                  | (_, k) :: xs => (KindCustomInd k, help2 xs)
-                                  end) ls)
-    | Array n k => pArray n (KindCustomInd k)
-    end.
-End KindInd.
+  Inductive Expr: Kind -> Type :=
+  | Var k: ty k -> Expr k
+  | Const k: type k -> Expr k
+  | UniBool: UniBoolOp -> Expr Bool -> Expr Bool
+  | CABool: CABoolOp -> list (Expr Bool) -> Expr Bool
+  | UniBit n1 n2: UniBitOp n1 n2 -> Expr (Bit n1) -> Expr (Bit n2)
+  | CABit n: CABitOp -> list (Expr (Bit n)) -> Expr (Bit n)
+  | BinBit n1 n2 n3: BinBitOp n1 n2 n3 -> Expr (Bit n1) -> Expr (Bit n2) -> Expr (Bit n3)
+  | BinBitBool n1 n2: BinBitBoolOp n1 n2 -> Expr (Bit n1) -> Expr (Bit n2) -> Expr Bool
+  | ITE k: Expr Bool -> Expr k -> Expr k -> Expr k
+  | Eq k: Expr k -> Expr k -> Expr Bool
+  | Kor k: list (Expr k) -> Expr k
+  | ReadStruct (ls: list (string * Kind)) (e: Expr (Struct ls)) (i: FinStruct ls): Expr (fieldK i)
+  | ReadArray n m k: Expr (Array n k) -> Expr (Bit m) -> Expr k
+  | ReadArrayConst n k: Expr (Array n k) -> FinArray n -> Expr k
+  | BuildArray k n (vals: FinArray n -> Expr k): Expr (Array n k)
+  | BuildStruct (ls: list (string * Kind)) (vals: forall i: FinStruct ls, Expr (fieldK i)): Expr (Struct ls)
+  | ToBit k (e: Expr k): Expr (Bit (size k))
+  | FromBit k (e: Expr (Bit (size k))): Expr k.
 
-Fixpoint type (k: Kind): Type :=
-  match k with
-  | Bool => bool
-  | Bit n => word n
-  | Struct skl => (fix helper skl : Type :=
-                     match skl with
-                     | nil => Empty_set
-                     | (_, k) :: xs => (type k * helper xs)%type
-                     end) skl (* @DiffTuple (string * Kind)%type (fun x => type (snd x)) skl *)
-  | Array n k' => SameTuple (type k') n
-  end.
+  Definition UpdateStruct ls (e: Expr (Struct ls)) (j: FinStruct ls) (v: Expr (fieldK j)): Expr (Struct ls) :=
+    BuildStruct _ (fun i => match FinStruct_dec _  j i return Expr (fieldK i) with
+                            | left pf => match pf in _ = Y return Expr (fieldK Y) with
+                                         | eq_refl => v
+                                         end
+                            | right _ => ReadStruct e i
+                            end).
 
-Section typeDec.
-  Lemma isEq k: forall (e1: type k) (e2: type k),
-      {e1 = e2} + {e1 <> e2}.
-  Proof.
-    induction k using KindCustomInd; simpl; intros.
-    - apply bool_dec.
-    - apply weq.
-    - induction ls.
-      + destruct e1.
-      + destruct a as (_, k).
-        destruct X as (indPf, helpPf).
-        apply (prod_dec indPf (IHls helpPf)).
-    - induction n.
-      + destruct e1.
-      + apply (prod_dec IHk IHn).
-  Defined.
-End typeDec.
+  Definition UpdateArrayConst n k (e: Expr (Array n k)) (i: FinArray n) (v: Expr k): Expr (Array n k) :=
+    BuildArray _ (fun j => match FinArray_dec _  i j return Expr k with
+                           | left pf => v
+                           | right _ => ReadArrayConst e j
+                           end).
 
-Definition forceOption A (o : option A) : match o with
-                                          | Some _ => A
-                                          | None => unit
-                                          end :=
-  match o with
-  | Some a => a
-  | None => tt
-  end.
+  Definition UpdateArray n k (e: Expr (Array n k)) m (i: Expr (Bit m)) (v: Expr k): Expr (Array n k) :=
+    BuildArray _ (fun j => ITE (Eq i (Const (Bit _) (natToWord _ (FinArray_to_nat _ j)))) v (ReadArrayConst e j)).
 
-Section FinStruct.
-  Fixpoint FinStruct (ls: list (string * Kind)) := match ls with
-                                                   | nil => Empty_set
-                                                   | x :: xs => (unit + FinStruct xs)%type
-                                                   end.
+  Section BitOps.
+    Definition castBits ni no (pf: ni = no) (e: Expr (Bit ni)) :=
+      nat_cast (fun n => Expr (Bit n)) pf e.
 
-  Fixpoint fieldType {ls: list (string * Kind)}: FinStruct ls -> type (Struct ls) -> Type :=
-    match ls return FinStruct ls -> type (Struct ls) -> Type with
-    | nil => fun i _ => match i with
-                        end
-    | (_, k) :: xs => fun i e => match i return Type with
-                                 | inl _ => type k
-                                 | inr y => @fieldType xs y (snd e)
-                                 end
-    end.
+    Definition Slt n (e1 e2: Expr (Bit (1 + n))) :=
+      Eq (Eq (UniBit (TruncMsb 1 n) e1) (UniBit (TruncMsb 1 n) e2)) (BinBitBool (LessThan _) e1 e2).
 
-  Fixpoint fieldVal (ls: list (string * Kind)): forall (i: FinStruct ls) (e: type (Struct ls)), fieldType i e :=
-    match ls return forall (i: FinStruct ls) (e: type (Struct ls)), fieldType i e with
-    | nil => fun i _ => match i with
-                        end
-    | (_, k) :: xs => fun i e => match i return @fieldType (_ :: xs) i e with
-                                 | inl _ => fst e
-                                 | inr y => @fieldVal xs y (snd e)
-                                 end
-    end.
+    Definition ConstExtract msb n lsb (e: Expr (Bit (msb + n + lsb))): Expr (Bit n) :=
+      UniBit (TruncLsb msb n) (UniBit (TruncMsb (msb + n) lsb) e).
 
-  Fixpoint getFinStructOption (s: string) (ls: list (string * Kind)): option (FinStruct ls) :=
-    match ls with
-    | nil => None
-    | (s', k) :: xs => match String.eqb s s' return option (FinStruct (_ :: xs)) with
-                       | true => Some (inl tt)
-                       | false => match getFinStructOption s xs return option (FinStruct (_ :: xs)) with
-                                  | None => None
-                                  | Some y => Some (inr y)
-                                  end
-                       end
-    end.
+    Definition OneExtend msb lsb (e: Expr (Bit lsb)): Expr (Bit (msb + lsb)) :=
+      BinBit (Concat msb lsb) (Const (Bit _) (wones msb)) e.
 
-  Definition getFinStruct s ls := forceOption (getFinStructOption s ls).
-End FinStruct.
+    Definition ZeroExtend msb lsb (e: Expr (Bit lsb)): Expr (Bit (msb + lsb)) :=
+      BinBit (Concat msb lsb) (Const (Bit _) (wzero msb)) e.
 
-Section FinArray.
-  Fixpoint FinArray n := match n with
-                         | 0 => Empty_set
-                         | S m => (unit + FinArray m)%type
-                         end.
+    Definition SignExtend msb lsb: Expr (Bit lsb) -> Expr (Bit (msb + lsb)).
+      refine
+        match lsb return Expr (Bit lsb) -> Expr (Bit (msb + lsb)) with
+        | 0 => fun _ => castBits _ (Const (Bit _) (wzero msb))
+        | S m => fun e => BinBit (Concat msb (S m)) (ITE (Eq (UniBit (TruncMsb 1 m) e)
+                                                            (Const (Bit _) (WO~0)%word))
+                                                         (Const (Bit _) (wzero msb))
+                                                         (Const (Bit _) (wones msb))) e
+        end; abstract lia.
+    Defined.
 
-  Fixpoint elementVal {k} {n}: forall (i: FinArray n) (e: type (Array n k)), type k :=
-    match n return forall (i: FinArray n) (e: type (Array n k)), type k with
-    | 0 => fun i _ => match i with
-                      end
-    | S m => fun i e => match i return type k with
-                        | inl _ => fst e
-                        | inr y => elementVal y (snd e)
-                        end
-    end.
+    Fixpoint replicate sz (e: Expr (Bit sz)) n : Expr (Bit (n * sz)) :=
+      match n return Expr (Bit (n * sz)) with
+      | 0 => Const (Bit _) WO
+      | S m => BinBit (Concat sz (m * sz)) e (replicate e m)
+      end.
+    
+    Definition OneExtendTruncLsb ni no (e: Expr (Bit ni)):
+      Expr (Bit no).
+      refine
+        match Compare_dec.lt_dec ni no with
+        | left isLt => castBits _ (@OneExtend (no - ni) ni e)
+        | right isGe => UniBit (TruncLsb (ni - no) no) (castBits _ e)
+        end; abstract lia.
+    Defined.
 
-  Fixpoint getFinArrayOption n k: option (FinArray n) :=
-    match n with
-    | 0 => None
-    | S m => match k return option (FinArray (S m)) with
-             | 0 => Some (inl tt)
-             | S k' => match getFinArrayOption m k' with
-                       | None => None
-                       | Some y => Some (inr y)
-                       end
-             end
-    end.
+    Definition ZeroExtendTruncLsb ni no (e: Expr (Bit ni)):
+      Expr (Bit no).
+      refine
+        match Compare_dec.lt_dec ni no with
+        | left isLt => castBits _ (@ZeroExtend (no - ni) ni e)
+        | right isGe => UniBit (TruncLsb (ni - no) no) (castBits _ e)
+        end; abstract lia.
+    Defined.
 
-  Definition getFinArray n k := forceOption (getFinArrayOption n k).
-End FinArray.
+    Definition SignExtendTruncLsb ni no (e: Expr (Bit ni)):
+      Expr (Bit no).
+      refine
+        match Compare_dec.lt_dec ni no with
+        | left isLt => castBits _ (@SignExtend (no - ni) ni e)
+        | right isGe => UniBit (TruncLsb (ni - no) no) (castBits _ e)
+        end; abstract lia.
+    Defined.
+    
+    Definition ZeroExtendTruncMsb ni no (e: Expr (Bit ni)):
+      Expr (Bit no).
+      refine
+        match Compare_dec.lt_dec ni no with
+        | left isLt => castBits _ (@ZeroExtend (no - ni) ni e)
+        | right isGe => UniBit (TruncMsb no (ni - no)) (castBits _ e)
+        end; abstract lia.
+    Defined.
+    
+    Definition SignExtendTruncMsb ni no (e: Expr (Bit ni)):
+      Expr (Bit no).
+      refine
+        match Compare_dec.lt_dec ni no with
+        | left isLt => castBits _ (@SignExtend (no - ni) ni e)
+        | right isGe => UniBit (TruncMsb no (ni - no)) (castBits _ e)
+        end; abstract lia.
+    Defined.
 
+    Definition isNotZero n (e: Expr (Bit n)) := FromBit Bool (UniBit (UOr n) e).
+    Definition isZero n (e: Expr (Bit n)) := UniBool Not (isNotZero e).
+    Definition isAllOnes n (e: Expr (Bit n)) := FromBit Bool (UniBit (UAnd n) e).
+
+    Fixpoint countLeadingZeros no ni: Expr (Bit ni) -> Expr (Bit no) :=
+      match ni return Expr (Bit ni) -> Expr (Bit no) with
+      | 0 => fun _ => Const (Bit _) (wzero _)
+      | S m => fun e =>
+                 ITE (Eq (UniBit (TruncMsb 1 m) e) (Const (Bit _) WO~0))
+                     (CABit Add [Const (Bit _) (natToWord _ 1);
+                                 @countLeadingZeros _ _ (UniBit (TruncLsb 1 m) e)])
+                     (Const (Bit _) (wzero _))
+      end.
+
+    Fixpoint countTrailingZeros no ni: Expr (Bit ni) -> Expr (Bit no) :=
+      match ni return Expr (Bit ni) -> Expr (Bit no) with
+      | 0 => fun _ => Const (Bit _) (wzero _)
+      | S m => fun e =>
+                 let eCast := castBits (eq_sym (Nat.add_1_r m)) e in
+                 ITE (Eq (UniBit (TruncLsb m 1) eCast) (Const (Bit _) WO~0))
+                        (CABit Add [Const (Bit _) (natToWord _ 1);
+                                    @countTrailingZeros _ _ (UniBit (TruncMsb m 1) eCast)])
+                     (Const (Bit _) (wzero _))
+      end.
+  End BitOps.
+End Phoas.
