Lib/Library.v
@@ -1,0 +1,555 @@
+Require Export Bool Ascii String List Psatz PeanoNat.
+Require Export Guru.Lib.Word Guru.Lib.WordProperties.
+
+Set Implicit Arguments.
+Set Asymmetric Patterns.
+
+Inductive Kind :=
+| Bool   : Kind
+| Bit    : nat -> Kind
+| Struct : list (string * Kind) -> Kind
+| Array  : nat -> Kind -> Kind.
+
+Axiom cheat: forall t, t.
+
+Section ProdDec.
+  Variable A B: Type.
+  Variable Adec: forall a1 a2: A, {a1 = a2} + {a1 <> a2}.
+  Variable Bdec: forall b1 b2: B, {b1 = b2} + {b1 <> b2}.
+
+  Definition prod_dec (x y: (A * B)%type): {x = y} + {x <> y} :=
+    match x, y with
+    | (a1, b1), (a2, b2) => match Adec a1 a2 with
+                            | left pf => match Bdec b1 b2 with
+                                         | left pf1 => left (match match pf in (_ = a) return (a = a1) with
+                                                                   | eq_refl => eq_refl
+                                                                   end in (_ = a) return ((a, b1) = (a2, b2)) with
+                                                             | eq_refl =>
+                                                                 match
+                                                                   match pf1 in (_ = a) return (a = b1) with
+                                                                   | eq_refl => eq_refl
+                                                                   end in (_ = a) return ((a2, a) = (a2, b2))
+                                                                 with
+                                                                 | eq_refl => eq_refl
+                                                                 end
+                                                             end)
+                                         | right pf1 =>
+                                             right (fun H : (a1, b1) = (a2, b2) =>
+                                                      match pf1 match H in (_ = a) return (b1 = snd a) with
+                                                              | eq_refl => eq_refl
+                                                              end return False
+                                                      with
+                                                      end)
+                                                          
+                                         end
+                            | right pf => right (fun H : (a1, b1) = (a2, b2) =>
+                                                   match
+                                                     pf match H in (_ = a) return (a1 = fst a) with
+                                                       | eq_refl => eq_refl
+                                                       end return False
+                                                   with
+                                                   end)
+                            end
+    end.
+End ProdDec.
+
+Section KindDec.
+  Local Notation contra k1 k2 := (right (fun H : k1 = k2 => match match H in (_ = a) return match a with
+                                                                                            | k1 => True
+                                                                                            | _ => False
+                                                                                            end with
+                                                                  | eq_refl => I
+                                                                  end return False with
+                                                            end)).
+
+  Fixpoint Kind_dec k1: forall k2: Kind, {k1 = k2} + {k1 <> k2} :=
+    match k1 with
+    | Bool => fun k2 => match k2 with
+                        | Bool => left eq_refl
+                        | Bit n => contra Bool (Bit n)
+                        | Struct ls => contra Bool (Struct ls)
+                        | Array n k => contra Bool (Array n k)
+                        end
+    | Bit n => fun k2 => match k2 with
+                         | Bool => contra (Bit n) Bool
+                         | Bit n1 => match Nat.eq_dec n n1 with
+                                     | left pf => left (match match pf in (_ = a) return (a = n) with
+                                                              | eq_refl => eq_refl
+                                                              end with
+                                                        | eq_refl => eq_refl
+                                                        end)
+                                     | right pf => right (fun H : Bit n = Bit n1 =>
+                                                            match pf match H in (_ = a) return (n = match a with
+                                                                                                    | Bit n0 => n0
+                                                                                                    | _ => n
+                                                                                                    end) with
+                                                                    | eq_refl => eq_refl
+                                                                    end return False with
+                                                            end)
+
+                                     end
+                         | Struct ls => contra (Bit n) (Struct ls)
+                         | Array n' k => contra (Bit n) (Array n' k)
+                         end
+    | Struct ls =>
+        fun k2 => match k2 with
+                  | Bool => contra (Struct ls) Bool
+                  | Bit n => contra (Struct ls) (Bit n)
+                  | Struct ls' => match list_eq_dec (prod_dec string_dec Kind_dec) ls ls' with
+                                  | left pf => left match match pf in (_ = a) return (a = ls) with
+                                                          | eq_refl => eq_refl
+                                                          end with
+                                                 | eq_refl => eq_refl
+                                                 end
+                                  | right n => right (fun H : Struct ls = Struct ls' =>
+                                                        match n match H in (_ = a) return (ls = match a with
+                                                                                                | Struct l => l
+                                                                                                | _ => ls
+                                                                                                end) with
+                                                                | eq_refl => eq_refl
+                                                                end return False with
+                                                        end)
+                                  end
+                  | Array n k => contra (Struct ls) (Array n k)
+                  end
+    | Array n k => fun k2 => match k2 with
+                             | Bool => contra (Array n k) Bool
+                             | Bit n' => contra (Array n k) (Bit n')
+                             | Struct ls => contra (Array n k) (Struct ls)
+                             | Array n' k' =>
+                                 match Nat.eq_dec n n' with
+                                 | left e =>
+                                     match Kind_dec k k' with
+                                     | left pf =>
+                                         left
+                                           match match e in (_ = a) return (a = n) with
+                                                 | eq_refl => eq_refl
+                                                 end with
+                                           | eq_refl =>
+                                               match match pf in (_ = a) return (a = k) with
+                                                     | eq_refl => eq_refl
+                                                     end with
+                                               | eq_refl => eq_refl
+                                               end
+                                           end
+                                     | right pf =>
+                                         right
+                                           (fun H : Array n k = Array n' k' =>
+                                              match pf match H in (_ = a) return (k = match a with
+                                                                                      | Array _ k0 => k0
+                                                                                      | _ => k
+                                                                                      end) with
+                                                      | eq_refl => eq_refl
+                                                      end return False with
+                                              end)
+                                     end
+                                 | right pf =>
+                                     right
+                                       (fun H : Array n k = Array n' k' =>
+                                          match pf match H in (_ = a) return (n = match a with
+                                                                                  | Array n1 _ => n1
+                                                                                  | _ => n
+                                                                                  end) with
+                                                  | eq_refl => eq_refl
+                                                  end return False with
+                                          end)
+                                 end
+                             end
+    end.
+End KindDec.
+
+Section DiffTuple.
+  Variable A: Type.
+  Variable Convert: A -> Type.
+  Fixpoint DiffTuple (ls: list A) := match ls return Type with
+                                     | nil => unit
+                                     | a :: xs => (Convert a * DiffTuple xs)%type
+                                     end.
+End DiffTuple.
+
+Section SameTuple.
+  Variable T: Type.
+  Fixpoint SameTuple n := match n return Type with
+                          | 0 => unit
+                          | S m => (T * SameTuple m)%type
+                          end.
+End SameTuple.
+
+Section KindInd.
+  Variable P: Kind -> Type.
+  Variable pBool: P Bool.
+  Variable pBit: forall n, P (Bit n).
+  Variable pStruct: forall ls: list (string * Kind), DiffTuple (fun x => P (snd x)) ls -> P (Struct ls).
+  Variable pArray: forall n k, P k -> P (Array n k).
+
+  Fixpoint KindCustomInd (k: Kind): P k :=
+    match k return P k with
+    | Bool => pBool
+    | Bit n => pBit n
+    | Struct ls => pStruct ls ((fix help2 ls :=
+                                  match ls return DiffTuple (fun x => P (snd x)) ls with
+                                  | nil => tt
+                                  | x :: xs => (KindCustomInd (snd x), help2 xs)
+                                  end) ls)
+    | Array n k => pArray n (KindCustomInd k)
+    end.
+End KindInd.
+
+Fixpoint type (k: Kind): Type :=
+  match k with
+  | Bool => bool
+  | Bit n => word n
+  | Struct ls => DiffTuple (fun x => type (snd x)) ls
+  | Array n k' => SameTuple (type k') n
+  end.
+
+Section typeDec.
+  Lemma isEq k: forall (e1: type k) (e2: type k),
+      {e1 = e2} + {e1 <> e2}.
+  Proof.
+    induction k using KindCustomInd; simpl; intros.
+    - apply bool_dec.
+    - apply weq.
+    - induction ls.
+      + left; destruct e1, e2; reflexivity.
+      + destruct X as (indPf, helpPf).
+        apply (prod_dec indPf (IHls helpPf)).
+    - induction n.
+      + left; destruct e1, e2; reflexivity.
+      + apply (prod_dec IHk IHn).
+  Defined.
+End typeDec.
+
+Definition forceOption A (o : option A) : match o with
+                                          | Some _ => A
+                                          | None => unit
+                                          end :=
+  match o with
+  | Some a => a
+  | None => tt
+  end.
+
+Section FinStruct.
+  Fixpoint FinStruct (ls: list (string * Kind)) := match ls with
+                                                   | nil => Empty_set
+                                                   | x :: xs => (unit + FinStruct xs)%type
+                                                   end.
+
+
+  Fixpoint FinStruct_dec (ls: list (string * Kind)): forall i j: FinStruct ls, {i = j} + {i <> j} :=
+    match ls return forall i j: FinStruct ls, {i = j} + {i <> j} with
+    | nil => fun i j => match i with
+                        end
+    | _ :: xs => fun i j => match i with
+                            | inl y => match j with
+                                       | inl z => match y, z with
+                                                  | tt, tt => left eq_refl
+                                                  end
+                                       | inr z => right (fun H : inl y = inr z =>
+                                                           match match H in (_ = a) return match a with
+                                                                                           | inl _ => True
+                                                                                           | inr _ => False
+                                                                                           end with
+                                                                 | eq_refl => I
+                                                                 end return False with
+                                                           end)
+                                       end
+                            | inr y => match j with
+                                       | inl z => right (fun H : inr y = inl z =>
+                                                           match match H in (_ = a) return match a with
+                                                                                           | inl _ => False
+                                                                                           | inr _ => True
+                                                                                           end with
+                                                                 | eq_refl => I
+                                                                 end return False with
+                                                           end)
+                                       | inr z => match FinStruct_dec xs y z with
+                                                  | left pf => left (f_equal _ pf)
+                                                  | right pf =>
+                                                      right
+                                                        (fun H : inr y = inr z =>
+                                                           match
+                                                             pf (f_equal (fun e => match e with
+                                                                                   | inl _ => y
+                                                                                   | inr f => f
+                                                                                   end) H) return False with
+                                                           end)
+                                                  end
+                                       end
+                            end
+    end.
+
+  Fixpoint fieldK {ls: list (string * Kind)}: FinStruct ls -> Kind :=
+    match ls return FinStruct ls -> Kind with
+    | nil => fun i => match i with
+                      end
+    | x :: xs => fun i => match i return Kind with
+                          | inl _ => snd x
+                          | inr y => @fieldK xs y
+                          end
+    end.
+
+  Fixpoint fieldType {ls: list (string * Kind)}: FinStruct ls -> type (Struct ls) -> Type :=
+    match ls return FinStruct ls -> type (Struct ls) -> Type with
+    | nil => fun i _ => match i with
+                        end
+    | x :: xs => fun i e => match i return Type with
+                            | inl _ => type (snd x)
+                            | inr y => @fieldType xs y (snd e)
+                            end
+    end.
+
+  Fixpoint fieldVal (ls: list (string * Kind)): forall (e: type (Struct ls)) (i: FinStruct ls), fieldType i e :=
+    match ls return forall (e: type (Struct ls)) (i: FinStruct ls), fieldType i e with
+    | nil => fun _ i => match i with
+                        end
+    | x :: xs => fun e i => match i return @fieldType (_ :: xs) i e with
+                            | inl _ => fst e
+                            | inr y => @fieldVal xs (snd e) y
+                            end
+    end.
+
+  Fixpoint getFinStructOption (s: string) (ls: list (string * Kind)): option (FinStruct ls) :=
+    match ls with
+    | nil => None
+    | x :: xs => match String.eqb s (fst x) return option (FinStruct (_ :: xs)) with
+                 | true => Some (inl tt)
+                 | false => match getFinStructOption s xs return option (FinStruct (_ :: xs)) with
+                            | None => None
+                            | Some y => Some (inr y)
+                            end
+                 end
+    end.
+
+  Definition getFinStruct s ls := forceOption (getFinStructOption s ls).
+
+  Section StructFuncTuple.
+    Variable ty: Kind -> Type.
+
+    Fixpoint getStructFuncToTuple ls: (forall i: FinStruct ls, ty (fieldK i)) -> DiffTuple (fun x => ty (snd x)) ls :=
+      match ls return (forall i: FinStruct ls, ty (fieldK i)) -> DiffTuple (fun x => ty (snd x)) ls with
+      | nil => fun _ => tt
+      | x :: xs => fun vals => (vals (inl tt), getStructFuncToTuple xs (fun i => vals (inr i)))
+      end.
+
+    Fixpoint getStructTupleToFunc ls: DiffTuple (fun x => ty (snd x)) ls -> forall i: FinStruct ls, ty (fieldK i) :=
+      match ls return DiffTuple (fun x => ty (snd x)) ls -> forall i: FinStruct ls, ty (fieldK i) with
+      | nil => fun _ i => match i with
+                          end
+      | x :: xs => fun vals i => match i with
+                                 | inl _ => fst vals
+                                 | inr y => getStructTupleToFunc xs (snd vals) y
+                                 end
+      end.
+  End StructFuncTuple.
+End FinStruct.
+
+Section FinArray.
+  Fixpoint FinArray n := match n with
+                         | 0 => Empty_set
+                         | S m => (unit + FinArray m)%type
+                         end.
+
+  Fixpoint FinArray_dec n: forall i j: FinArray n, {i = j} + {i <> j} :=
+    match n return forall i j: FinArray n, {i = j} + {i <> j} with
+    | 0 => fun i j => match i with
+                        end
+    | S m => fun i j => match i with
+                        | inl y => match j with
+                                   | inl z => match y, z with
+                                              | tt, tt => left eq_refl
+                                              end
+                                   | inr z => right (fun H : inl y = inr z =>
+                                                       match match H in (_ = a) return match a with
+                                                                                       | inl _ => True
+                                                                                       | inr _ => False
+                                                                                       end with
+                                                             | eq_refl => I
+                                                             end return False with
+                                                       end)
+                                   end
+                        | inr y => match j with
+                                   | inl z => right (fun H : inr y = inl z =>
+                                                       match match H in (_ = a) return match a with
+                                                                                       | inl _ => False
+                                                                                       | inr _ => True
+                                                                                       end with
+                                                             | eq_refl => I
+                                                             end return False with
+                                                       end)
+                                   | inr z => match FinArray_dec m y z with
+                                              | left pf => left (f_equal _ pf)
+                                              | right pf =>
+                                                  right
+                                                    (fun H : inr y = inr z =>
+                                                       match
+                                                         pf (f_equal (fun e => match e with
+                                                                               | inl _ => y
+                                                                               | inr f => f
+                                                                               end) H) return False with
+                                                       end)
+                                              end
+                                   end
+                        end
+    end.
+
+  Fixpoint FinArray_to_nat n: FinArray n -> nat :=
+    match n return FinArray n -> nat with
+    | 0 => fun i => match i with
+                    end
+    | S m => fun i => match i with
+                      | inl _ => m
+                      | inr y => FinArray_to_nat _ y
+                      end
+    end.
+
+  Fixpoint elementVal {k} {n}: forall (e: type (Array n k)) (i: FinArray n), type k :=
+    match n return forall (e: type (Array n k)) (i: FinArray n), type k with
+    | 0 => fun _ i => match i with
+                      end
+    | S m => fun e i => match i return type k with
+                        | inl _ => fst e
+                        | inr y => elementVal (snd e) y
+                        end
+    end.
+
+  Fixpoint getFinArrayOption n k: option (FinArray n) :=
+    match n with
+    | 0 => None
+    | S m => match k return option (FinArray (S m)) with
+             | 0 => Some (inl tt)
+             | S k' => match getFinArrayOption m k' with
+                       | None => None
+                       | Some y => Some (inr y)
+                       end
+             end
+    end.
+
+  Definition getFinArray n k := forceOption (getFinArrayOption n k).
+
+  Section ArrayFuncTuple.
+    Variable ty: Kind -> Type.
+    Variable k: Kind.
+
+    Fixpoint getArrayFuncToTuple n: (FinArray n -> ty k) -> SameTuple (ty k) n :=
+      match n return (FinArray n -> ty k) -> SameTuple (ty k) n with
+      | 0 => fun _ => tt
+      | S m => fun vals => (vals (inl tt), getArrayFuncToTuple m (fun i => vals (inr i)))
+      end.
+
+    Fixpoint getArrayTupleToFunc n: SameTuple (ty k) n -> forall i: FinArray n, ty k :=
+      match n return SameTuple (ty k) n -> forall i: FinArray n, ty k with
+      | 0 => fun _ i => match i with
+                        end
+      | S m => fun vals i => match i with
+                             | inl _ => fst vals
+                             | inr y => getArrayTupleToFunc m (snd vals) y
+                             end
+      end.
+  End ArrayFuncTuple.
+End FinArray.
+
+Section DiffTupleDefault.
+  Variable A: Type.
+  Variable ConvertType: A -> Type.
+  Variable convertVal: forall a, ConvertType a.
+
+  Fixpoint DiffTupleDefault ls :=
+    match ls return DiffTuple ConvertType ls with
+    | nil => tt
+    | x :: xs => (convertVal x, DiffTupleDefault xs)
+    end.
+End DiffTupleDefault.
+
+Section SameTupleDefault.
+  Variable A: Type.
+  Variable val: A.
+
+  Fixpoint SameTupleDefault n :=
+    match n return SameTuple A n with
+    | 0 => tt
+    | S m => (val, SameTupleDefault m)
+    end.
+End SameTupleDefault.
+
+Fixpoint getDefault (k: Kind): type k :=
+  match k return type k with
+  | Bool => false
+  | Bit n => wzero n
+  | Struct ls => DiffTupleDefault (fun x => type (snd x)) (fun x => getDefault (snd x)) ls
+  | Array n k' => SameTupleDefault (getDefault k') n
+  end.
+
+Fixpoint size (k: Kind) :=
+  match k with
+  | Bool => 1
+  | Bit n => n
+  | Struct ls => (fix help ls :=
+                    match ls with
+                    | nil => 0
+                    | x :: xs => size (@fieldK (x :: xs) (inl tt)) + help xs
+                    end) ls
+  | Array n k => n * size k
+  end.
+
+Section ToBit.
+  Variable toBit: forall k, type k -> word (size k).
+
+  Fixpoint evalStructToBit ls: forall (f: forall (i: FinStruct ls), type (fieldK i)),
+      word (size (Struct ls)) :=
+    match ls return forall (f: forall (i: FinStruct ls), type (fieldK i)),
+        word (size (Struct ls)) with
+    | nil => fun _ => WO
+    | _ :: xs => fun f => wcombine (toBit _ (f (inl tt)))
+                            (@evalStructToBit xs (fun (x: FinStruct xs) => (f (inr x))))
+    end.
+
+  Fixpoint evalArrayToBit k n: forall (f: forall (i: FinArray n), type k),
+      word (size (Array n k)) :=
+    match n return forall (f: forall (i: FinArray n), type k),
+        word (size (Array n k)) with
+    | 0 => fun _ => WO
+    | S m => fun f => wcombine (toBit _ (f (inl tt)))
+                        (@evalArrayToBit k m (fun (x: FinArray m) => (f (inr x))))
+    end.
+End ToBit.
+
+Fixpoint evalToBit k: type k -> word (size k) :=
+  match k return type k -> word (size k) with
+  | Bool => fun v => if v then WO~1 else WO~0
+  | Bit n => fun v => v
+  | Struct ls => fun v => evalStructToBit evalToBit _ (getStructTupleToFunc _ _ v)
+  | Array n k => fun v => evalArrayToBit evalToBit _ _ (getArrayTupleToFunc _ _ _ v)
+  end.
+
+Section FromBit.
+  Variable fromBit: forall k, word (size k) -> type k.
+
+  Fixpoint evalBitToStruct ls: word (size (Struct ls)) -> forall (i: FinStruct ls), type (fieldK i) :=
+    match ls return word (size (Struct ls)) -> forall (i: FinStruct ls), type (fieldK i) with
+    | nil => fun _ i => match i with
+                        end
+    | x :: xs => fun v i => match i return type (@fieldK (x :: xs) i) with
+                            | inl _ => fromBit _ (@truncMsb (size (@fieldK (x :: xs) (inl tt))) _ v)
+                            | inr y => evalBitToStruct _ (@truncLsb (size (Struct xs)) _ v) y
+                            end
+    end.
+
+  Fixpoint evalBitToArray k n: word (size (Array n k)) -> forall (i: FinArray n), type k :=
+    match n return word (size (Array n k)) -> forall (i: FinArray n), type k with
+    | 0 => fun _ i => match i with
+                      end
+    | S m => fun v i => match i return type k with
+                        | inl _ => fromBit _ (@truncMsb (size k) _ v)
+                        | inr y => evalBitToArray _ _ (@truncLsb (size (Array m k)) _ v) y
+                        end
+    end.
+End FromBit.
+
+Fixpoint evalFromBit k: word (size k) -> type k :=
+  match k return word (size k) -> type k with
+  | Bool => fun v => if weq v WO~1 then true else false
+  | Bit n => fun v => v
+  | Struct ls => fun v => getStructFuncToTuple _ _ (evalBitToStruct evalFromBit _ v)
+  | Array n k => fun v => getArrayFuncToTuple _ _ _ (evalBitToArray evalFromBit _ _ v)
+  end.
