Lib/Word.v
@@ -1,6 +1,5 @@
 Require Import Coq.ZArith.BinIntDef Coq.ZArith.BinInt Coq.ZArith.Zdiv Psatz.
 
-
 Definition minimize_eq_proof{A: Type}(eq_dec: forall (x y: A), {x = y} + {x <> y}){x y: A}    (pf: x = y): x = y :=
   match eq_dec x y with
   | left p => p
